qtesla/code/Hacl.Impl.QTesla.TargetConfig.fsti
@@ -1,0 +1,5 @@
+module Hacl.Impl.QTesla.TargetConfig
+
+[@ CIfDef ]
+inline_for_extraction
+val isProvable: bool
